src/Spec/Abstraction.v
@@ -17,6 +17,25 @@ Section Abstraction.
              (spec: relation AState AState T) :=
     absr;; p ---> v <- spec; absr;; pure v.
 
+  Theorem refine_unfolded_iff T
+          (p: relation CState CState T)
+          (spec: relation AState AState T) :
+    (forall s s__a, absr s__a s tt ->
+             forall s' v, p s s' v ->
+                     exists s__a', spec s__a s__a' v /\
+                            absr s__a' s' tt) <->
+    refines p spec.
+  Proof.
+    unfold refines, rimpl, and_then, pure; split.
+    - propositional.
+      destruct o1.
+      eapply H in H0; eauto; propositional.
+      eauto 10.
+    - intros. edestruct H; eauto. propositional.
+      destruct o1.
+      eauto 10.
+  Qed.
+
   Theorem refine_unfolded T
           (p: relation CState CState T)
           (spec: relation AState AState T) :
@@ -25,12 +44,7 @@ Section Abstraction.
                      exists s__a', spec s__a s__a' v /\
                             absr s__a' s' tt) ->
     refines p spec.
-  Proof.
-    unfold refines, rimpl, and_then, pure; propositional.
-    destruct o1.
-    eapply H in H0; eauto; propositional.
-    eauto 10.
-  Qed.
+  Proof. eapply refine_unfolded_iff. Qed.
 
   (* define refinement as transforming an abstract specification to a concrete
   one (a program satisfying the abstract spec should satisfy the concrete spec
@@ -116,4 +130,27 @@ Theorem refines_trans State1 State2 abs T
   refines abs (r1;; r2) (r1';; r2').
 Proof.
   auto using refines_trans_bind.
+Qed.
+
+Theorem refines_star State1 State2 abs T
+        (r1: relation State1 State1 T)
+        (r2: relation State2 State2 T) :
+  refines abs r1 r2 ->
+  refines abs (seq_star r1) (seq_star r2).
+Proof.
+  unfold refines. intros Hr.
+  rew simulation_seq_value; auto.
+Qed.
+
+Theorem refines_or State1 State2 abs T
+        (r1 r1': relation State1 State1 T)
+        (r2 r2': relation State2 State2 T) :
+  refines abs r1 r2 ->
+  refines abs r1' r2' ->
+  refines abs (r1 + r1') (r2 + r2').
+Proof.
+  unfold refines. intros Hr Hr'.
+  repeat rew bind_dist_r.
+  repeat rew bind_dist_l.
+  rew Hr. rew Hr'.
 Qed.
